serialize_list_up_to

src/lowparse/LowParse.Spec.ListUpTo.fst
@@ -81,7 +81,7 @@ let parse_list_up_to_payload
   (x: t)
 : Tot (parser (parse_list_up_to_kind k) (parse_list_up_to_payload_t cond fuel x))
 = if cond x
-  then weaken (parse_list_up_to_kind k) (parse_ret ())
+  then weaken (parse_list_up_to_kind k) parse_empty
   else ptail
 
 let rec parse_list_up_to_fuel
@@ -371,3 +371,164 @@ let parse_list_up_to_eq
       parse_list_up_to'_eq cond p fuel' b' ;
       parse_list_up_to_fuel_ext cond p prf (fuel - 1) fuel' b'
     end
+
+(* serializer *)
+
+let serialize_list_up_to_payload
+  (#t: Type)
+  (cond: (t -> Tot bool))
+  (fuel: nat)
+  (k: parser_kind { k.parser_kind_subkind <> Some ParserConsumesAll })
+  (#ptail: parser (parse_list_up_to_kind k) (parse_list_up_to_fuel_t cond fuel))
+  (stail: serializer ptail)
+  (x: t)
+: Tot (serializer (parse_list_up_to_payload cond fuel k ptail x))
+= if cond x
+  then serialize_weaken (parse_list_up_to_kind k) serialize_empty
+  else stail
+
+let synth_list_up_to_fuel_recip
+  (#t: Type)
+  (cond: (t -> Tot bool))
+  (fuel: nat)
+  (xy: parse_list_up_to_fuel_t cond (fuel + 1))
+: Tot (dtuple2 t (parse_list_up_to_payload_t cond fuel))
+= let (l, z) = xy in
+  match l with
+  | [] -> (| z, () |)
+  | x :: y -> (| x, ((y <: llist (parse_filter_refine (negate_cond cond)) fuel), z) |)
+
+let synth_list_up_to_fuel_inverse
+  (#t: Type)
+  (cond: (t -> Tot bool))
+  (fuel: nat)
+: Lemma
+  (synth_inverse (synth_list_up_to_fuel cond fuel) (synth_list_up_to_fuel_recip cond fuel))
+  [SMTPat (synth_inverse (synth_list_up_to_fuel cond fuel) (synth_list_up_to_fuel_recip cond fuel))]
+= ()
+
+let rec serialize_list_up_to_fuel
+  (#k: parser_kind)
+  (#t: Type)
+  (cond: (t -> Tot bool))
+  (#p: parser k t)
+  (s: serializer p { k.parser_kind_subkind == Some ParserStrong })
+  (fuel: nat)
+: Tot (serializer (parse_list_up_to_fuel cond p fuel))
+  (decreases fuel)
+= if fuel = 0
+  then fail_serializer (parse_list_up_to_kind k) (parse_list_up_to_fuel_t cond fuel) (fun _ -> ())
+  else
+    serialize_synth
+      (parse_dtuple2
+        (weaken (parse_list_up_to_kind k) p)
+        #(parse_list_up_to_kind k)
+        #(parse_list_up_to_payload_t cond (fuel - 1))
+        (parse_list_up_to_payload cond (fuel - 1) k (parse_list_up_to_fuel cond p (fuel - 1))))
+      (synth_list_up_to_fuel cond (fuel - 1))
+      (serialize_dtuple2
+        (serialize_weaken (parse_list_up_to_kind k) s)
+        #(parse_list_up_to_kind k)
+        #(parse_list_up_to_payload_t cond (fuel - 1))
+        #(parse_list_up_to_payload cond (fuel - 1) k (parse_list_up_to_fuel cond p (fuel - 1)))
+        (serialize_list_up_to_payload cond (fuel - 1) k (serialize_list_up_to_fuel cond s (fuel - 1))))
+      (synth_list_up_to_fuel_recip cond (fuel - 1))
+      ()
+
+let serialize_list_up_to_fuel_eq
+  (#k: parser_kind)
+  (#t: Type)
+  (cond: (t -> Tot bool))
+  (#p: parser k t)
+  (s: serializer p { k.parser_kind_subkind == Some ParserStrong })
+  (fuel: nat)
+  (xy: parse_list_up_to_fuel_t cond fuel)
+: Lemma
+  (serialize (serialize_list_up_to_fuel cond s fuel) xy `Seq.equal` (
+    let (l, z) = xy in
+    match l with
+    | [] -> serialize s z
+    | x :: y -> serialize s x `Seq.append` serialize (serialize_list_up_to_fuel cond s (fuel - 1)) ((y <: llist (parse_filter_refine (negate_cond cond)) (fuel - 1)), z)
+  ))
+= 
+  serialize_synth_eq
+    (parse_dtuple2
+      (weaken (parse_list_up_to_kind k) p)
+      #(parse_list_up_to_kind k)
+      #(parse_list_up_to_payload_t cond (fuel - 1))
+      (parse_list_up_to_payload cond (fuel - 1) k (parse_list_up_to_fuel cond p (fuel - 1))))
+    (synth_list_up_to_fuel cond (fuel - 1))
+    (serialize_dtuple2
+      (serialize_weaken (parse_list_up_to_kind k) s)
+      #(parse_list_up_to_kind k)
+      #(parse_list_up_to_payload_t cond (fuel - 1))
+      #(parse_list_up_to_payload cond (fuel - 1) k (parse_list_up_to_fuel cond p (fuel - 1)))
+      (serialize_list_up_to_payload cond (fuel - 1) k (serialize_list_up_to_fuel cond s (fuel - 1))))
+    (synth_list_up_to_fuel_recip cond (fuel - 1))
+    ()
+    xy;
+  serialize_dtuple2_eq' 
+    (serialize_weaken (parse_list_up_to_kind k) s)
+    #(parse_list_up_to_kind k)
+    #(parse_list_up_to_payload_t cond (fuel - 1))
+    #(parse_list_up_to_payload cond (fuel - 1) k (parse_list_up_to_fuel cond p (fuel - 1)))
+    (serialize_list_up_to_payload cond (fuel - 1) k (serialize_list_up_to_fuel cond s (fuel - 1))) 
+    (synth_list_up_to_fuel_recip cond (fuel - 1) xy)
+
+let serialize_list_up_to'
+  (#k: parser_kind)
+  (#t: Type)
+  (cond: (t -> Tot bool))
+  (#p: parser k t)
+  (s: serializer p { k.parser_kind_subkind == Some ParserStrong })
+: Tot (bare_serializer (parse_list_up_to_t cond))
+= fun xy ->
+  serialize (serialize_list_up_to_fuel cond s (L.length (fst xy) + 1)) (fst xy, snd xy)
+
+let serialize_list_up_to_correct
+  (#k: parser_kind)
+  (#t: Type)
+  (cond: (t -> Tot bool))
+  (#p: parser k t)
+  (prf: consumes_if_not_cond cond p)
+  (s: serializer p { k.parser_kind_subkind == Some ParserStrong })
+  (xy: parse_list_up_to_t cond)
+: Lemma
+  (
+    let sq = serialize_list_up_to' cond s xy in
+    parse (parse_list_up_to cond p prf) sq == Some (xy, Seq.length sq)
+  )
+= let sq = serialize_list_up_to' cond s xy in
+  let fuel' = close_parse_list_up_to sq in
+  let fuel = L.length (fst xy) + 1 in
+  parse_list_up_to'_eq cond p fuel' sq;
+  parse_list_up_to_fuel_length cond p prf fuel sq;
+  parse_list_up_to_fuel_indep cond p fuel sq (fst xy, snd xy) (Seq.length sq) fuel'
+
+let serialize_list_up_to
+  (#k: parser_kind)
+  (#t: Type)
+  (cond: (t -> Tot bool))
+  (#p: parser k t)
+  (prf: consumes_if_not_cond cond p)
+  (s: serializer p { k.parser_kind_subkind == Some ParserStrong })
+: Tot (serializer (parse_list_up_to cond p prf))
+= Classical.forall_intro (serialize_list_up_to_correct cond prf s);
+  serialize_list_up_to' cond s
+
+let serialize_list_up_to_eq
+  (#k: parser_kind)
+  (#t: Type)
+  (cond: (t -> Tot bool))
+  (#p: parser k t)
+  (prf: consumes_if_not_cond cond p)
+  (s: serializer p { k.parser_kind_subkind == Some ParserStrong })
+  (xy: parse_list_up_to_t cond)
+: Lemma
+  (serialize (serialize_list_up_to cond prf s) xy == (
+    let (l, z) = xy in
+    match l with
+    | [] -> serialize s z
+    | x :: y -> serialize s x `Seq.append` serialize (serialize_list_up_to cond prf s) (y, z)
+  ))
+= serialize_list_up_to_fuel_eq cond s (L.length (fst xy) + 1) (fst xy, snd xy)
